\documentclass{article}
\usepackage{graphicx}
\usepackage{geometry}
\usepackage{amsmath}

\geometry{margin=0.8in}

\title{THU-DiscreteMathmatics-Homework-2}
\author{He Yuhui\quad 2022012050}
\date{September 2024}

\begin{document}

\maketitle

\section{Homework}

\subsection{Transform to Polish Notation}

\begin{itemize}
    \item[1] $\to\vee PQ\vee RS$
    \item[2] $\leftrightarrow\wedge\lnot PR\wedge PQ$
    \item[3] $\vee\vee\lnot\lnot P\wedge WR\lnot Q$
    \item[4] $\wedge P\to Q\lnot R$
\end{itemize}

\subsection{Prove}

\begin{itemize}
    \item[1] We have

    $$
        \begin{aligned}
            &P\to Q\\
            (\textbf{Implication Equivalence}) \Leftrightarrow\;&\lnot P\vee Q\\
            (\textbf{Commutative}) \Leftrightarrow\;&Q\vee\lnot P\\
            (\textbf{Double Negation}) \Leftrightarrow\;&\lnot(\lnot Q)\vee(\lnot P)\\
            (\textbf{Implication Equivalence}) \Leftrightarrow\;&\lnot Q\to\lnot P
        \end{aligned}
    $$

    \item[2] We have

    $$
        \begin{aligned}
            &((P\to \lnot Q)\to(Q\to \lnot P))\wedge R\\
            (\textbf{Implication Equivalence}) \Leftrightarrow\;&((\lnot P\vee\lnot Q)\to(\lnot Q\vee\lnot P))\wedge R\\
            (\textbf{Implication Equivalence}) \Leftrightarrow\;&(\lnot(\lnot P\vee\lnot Q)\vee(\lnot Q\vee\lnot P))\wedge R\\
            (\textbf{De Morgan Law}) \Leftrightarrow\;&((P\wedge Q)\vee \lnot(Q\wedge P))\wedge R\\
            (\textbf{Commutative}) \Leftrightarrow\;&((P\wedge Q)\vee \lnot(P\wedge Q))\wedge R\\
            (\textbf{Use}\;S\;\textbf{to denote}\;P\wedge Q) \Leftrightarrow\;&(S\vee\lnot S)\wedge R\\
            (\textbf{Negation}) \Leftrightarrow\;&\mathsf{T}\wedge R\\
            (\textbf{Absorption}) \Leftrightarrow\;& R
        \end{aligned}
    $$

    \item[3] We have

    $$
        \begin{aligned}
            &(P\leftrightarrow Q)\leftrightarrow((P\wedge\lnot Q)\vee (Q\wedge\lnot P))\\
            (\textbf{Equivalence Law}) \Leftrightarrow\;&((P\to Q)\wedge(Q\to P))\leftrightarrow ((P\wedge\lnot Q)\vee (Q\wedge\lnot P))\\
            (\textbf{Implication Equivalence}) \Leftrightarrow\;&((\lnot P\vee Q)\wedge(\lnot Q\vee P))\leftrightarrow((P\wedge\lnot Q)\vee (Q\wedge\lnot P))\\
            (\textbf{De Morgan Law}) \Leftrightarrow\;&\lnot((P\wedge\lnot Q)\vee (Q\wedge\lnot P))\leftrightarrow ((P\wedge\lnot Q)\vee (Q\wedge\lnot P))\\
            (\textbf{Use}\;R\;\textbf{to denote}\;(P\wedge\lnot Q)\vee (Q\wedge\lnot P)) \Leftrightarrow\;& \lnot R\leftrightarrow R\\
            (\textbf{Complement Law}) \Leftrightarrow\;&\mathsf{F}\\
            (\textbf{Negation}) \Leftrightarrow\;& P\wedge\lnot P
        \end{aligned}
    $$

    \item[4] We have

    $$
        \begin{aligned}
            & P\to(Q\to R)\\
            (\textbf{Implication Equivalence}) \Leftrightarrow\;&P\to (\lnot Q\vee R)\\
            (\textbf{Implication Equivalence}) \Leftrightarrow\;&\lnot P\vee(\lnot Q\vee R)\\
            (\textbf{Associative}) \Leftrightarrow\;&(\lnot P\vee\lnot Q)\vee R\\
            (\textbf{De Morgan Law}) \Leftrightarrow\;&\lnot(P\wedge Q)\vee R\\
            (\textbf{Implication Equivalence}) \Leftrightarrow\;&(P\wedge Q)\to R
        \end{aligned}
    $$

\end{itemize}

\subsection{Write the Statement of  $A$ and $B$}

\begin{itemize}
    \item[$A$] We have

    $$
        \begin{aligned}
            A&=(\lnot P\wedge\lnot Q)\\
            &=\lnot(P\vee Q)
        \end{aligned}
    $$

    \item[$B$] We have

    $$
        \begin{aligned}
            B&=\lnot(P\wedge\lnot Q)\\
            &=\lnot P\vee Q
        \end{aligned}
    $$
    
\end{itemize}

\subsection{Using $\uparrow$ and $\downarrow$ to denote $\lnot$, $\wedge$, $\vee$ and $\to$}

We know that

$$
    A\uparrow B\Leftrightarrow \lnot(A\wedge B),\quad A\downarrow B\Leftrightarrow \lnot(A\vee B)
$$

\begin{itemize}
    \item[$\lnot$] We have

    $$
        \begin{aligned}
            \lnot A&=\lnot(A\wedge A)=A\uparrow A\\
            \lnot A&=\lnot(A\vee A)=A\downarrow A
        \end{aligned}
    $$

    \item[$\wedge$] We have

    $$
        \begin{aligned}
            A\wedge B&=\lnot\lnot(A\wedge B)\\
            &=\lnot(A\uparrow B)\\
            &=(A\uparrow B)\uparrow(A\uparrow B)\\
            A\wedge B&=\lnot(\lnot A\vee\lnot B)\\
            &=(\lnot A)\downarrow(\lnot B)\\
            &=(A\downarrow A)\downarrow(B\downarrow B)
        \end{aligned}
    $$

    \item[$\vee$] We have

    $$
        \begin{aligned}
            A\vee B&=\lnot(\lnot A\wedge\lnot B)\\
            &=(\lnot A)\uparrow(\lnot B)\\
            &=(A\uparrow A)\uparrow(B\uparrow B)\\
            A\vee B&=\lnot\lnot(A\vee B)\\
            &=\lnot(A\downarrow B)\\
            &=(A\downarrow B)\downarrow(A\downarrow B)
        \end{aligned}
    $$

    \item[$\to$] We have

    $$
        \begin{aligned}
            A\to B&=\lnot A\vee B\\
            &=\lnot(A\wedge \lnot B)\\
            &=A\uparrow(\lnot B)\\
            &=A\uparrow(B\uparrow B)\\
            A\to B&=\lnot A\vee B\\
            &=\lnot\lnot(\lnot A\vee B)\\
            &=\lnot(\lnot A\downarrow B)\\
            &=\lnot((A\downarrow A)\downarrow B)\\
            &=((A\downarrow A)\downarrow B)\downarrow((A\downarrow A)\downarrow B)
        \end{aligned}
    $$
\end{itemize}

\end{document}
